Added definition solvable + roadmap

src/computability/problem.lean
@@ -2,6 +2,7 @@ import tactic
 import computability.primrec
 import computability.reduce
 import computability.tm_to_partrec
+import computability.turing_machine
 import data.zmod.basic
 import data.equiv.list
 import data.list.basic
@@ -12,7 +13,7 @@ open function
 namespace option
 def domain_add_option { α β : Type } : ( α → option β ) → ( option α → option β ) := begin
   intros f a,
-  cases a, 
+  cases a,
   use none,
   use f a,
 end
@@ -27,27 +28,31 @@ end option
 
 namespace problem
 
-structure problem (α : Type*) [primcodable α] :=
+structure problem (α : Type*) [encodable α] :=
 (yesinstance : α → Prop)
-
-namespace primcodable
-instance nat : primcodable ℕ := {
-  prim := nat.primrec.succ,
-  ..encodable.nat,
-}
-end primcodable
 
 def is_even : problem ℕ := {
   yesinstance := λ n, n%2 = 0,
-  ..primcodable.nat,
+  ..encodable.nat,
 }
 
 def is_odd : problem ℕ := {
   yesinstance := λ n, n%2 = 1,
-  ..primcodable.nat,
+  ..encodable.nat,
 }
 
-def many_one_reducible {α β} [primcodable α] [primcodable β] (P : problem α) (Q : problem β) :=
+def partrec {α σ} [encodable α] [encodable σ]
+  (f : α →. σ) := nat.partrec (λ n,
+  roption.bind (encodable.decode α n) (λ a, (f a).map encodable.encode))
+
+def computable {α σ} [encodable α] [encodable σ] (f : α → σ) := partrec (f : α →. σ)
+
+namespace computable
+protected theorem id {α : Type*} [encodable α]: computable (@id α) := sorry
+end computable
+
+
+def many_one_reducible {α β} [encodable α] [encodable β] (P : problem α) (Q : problem β) :=
 ∃ f : α → β, computable f ∧ ∀ a, P.yesinstance a ↔ Q.yesinstance (f a)
 -- ∃ f : α → β, computable f ∧ ∀ a, p a ↔ q (f a)
 
@@ -83,13 +88,13 @@ lemma is_odd_red_to_is_even: is_odd ≤₀ is_even := begin
 end
 
 @[refl]
-lemma many_one_reducible_refl {α} [primcodable α] (P : problem α) :
+lemma many_one_reducible_refl {α} [encodable α] (P : problem α) :
   P ≤₀ P := ⟨id, computable.id, by simp⟩
 
-@[trans]
-theorem many_one_reducible.trans {α β γ} [primcodable α] [primcodable β] [primcodable γ] {P : problem α} {Q : problem β} {R : problem γ} : P ≤₀ Q → Q ≤₀ R → P ≤₀ R
-| ⟨f, c₁, h₁⟩ ⟨g, c₂, h₂⟩ := ⟨g ∘ f, c₂.comp c₁,
-  λ a, ⟨λ h, by rwa [←h₂, ←h₁], λ h, by rwa [h₁, h₂]⟩⟩
+-- @[trans]
+-- theorem many_one_reducible.trans {α β γ} [encodable α] [encodable β] [encodable γ] {P : problem α} {Q : problem β} {R : problem γ} : P ≤₀ Q → Q ≤₀ R → P ≤₀ R
+-- | ⟨f, c₁, h₁⟩ ⟨g, c₂, h₂⟩ := ⟨g ∘ f, c₂.comp c₁,
+--   λ a, ⟨λ h, by rwa [←h₂, ←h₁], λ h, by rwa [h₁, h₂]⟩⟩
 
 -- structure algorithm {α : Type*} [primcodable α] (P : problem α) :=
 -- (K : Type*)
@@ -107,26 +112,26 @@ inductive propositional_formula (α : Type*)
 
 -- Postfix territory
 namespace propositional_formula
-def to_postfix : (propositional_formula ℕ) → list ℕ 
+def to_postfix : (propositional_formula ℕ) → list ℕ
 | (atom a) := [a+3]
 | (conj a b) :=  (to_postfix a) ++ (to_postfix b) ++ [1]
 | (disj a b) :=  (to_postfix a) ++ (to_postfix b) ++ [2]
 | (not a) := (to_postfix a) ++ [0]
 
-def from_postfix2' : list ℕ → list ( propositional_formula ℕ ) → list ℕ × list ( propositional_formula ℕ ) 
+def from_postfix' : list ℕ → list ( propositional_formula ℕ ) → list ℕ × list ( propositional_formula ℕ )
 | [] [f] := ([],[f])
 | [] m := ([],[])
-| (0::l) (f::m) := from_postfix2' l ((not f)::m) 
+| (0::l) (f::m) := from_postfix' l ((not f)::m)
 | (0::l) nil := ([],[])
-| (1::l) (f::(g::m)) := from_postfix2' l ((conj g f)::m) 
+| (1::l) (f::(g::m)) := from_postfix' l ((conj g f)::m)
 | (1::l) m := ([],[])
-| (2::l) (f::(g::m)) := from_postfix2' l ((disj g f)::m)
+| (2::l) (f::(g::m)) := from_postfix' l ((disj g f)::m)
 | (2::l) m := ([],[])
-| ((b+3)::l) m := from_postfix2' l ((atom b)::m)
+| ((b+3)::l) m := from_postfix' l ((atom b)::m)
 
-def from_postfix2 : list ℕ → option ( propositional_formula ℕ ) := λ l, list.head' ( from_postfix2' l [] ).2
+def from_postfix : list ℕ → option ( propositional_formula ℕ ) := λ l, list.head' ( from_postfix' l [] ).2
 
-lemma from_to_postfix_id_aux (φ:propositional_formula ℕ) : ∀ l₁:list ℕ, ∀ l₂:list (propositional_formula ℕ), from_postfix2' ( φ.to_postfix ++ l₁ ) l₂ = from_postfix2' l₁ ( φ :: l₂ ) :=
+lemma from_to_postfix_id_aux (φ:propositional_formula ℕ) : ∀ l₁:list ℕ, ∀ l₂:list (propositional_formula ℕ), from_postfix' ( φ.to_postfix ++ l₁ ) l₂ = from_postfix' l₁ ( φ :: l₂ ) :=
 begin
   induction φ, {
     intros l₁ l₂,
@@ -135,30 +140,30 @@ begin
     intros l₁ l₂,
     specialize φ_ih_a (φ_b.to_postfix ++ (1 :: l₁) ) l₂,
     specialize φ_ih_b (1 :: l₁) (φ_a :: l₂),
-    calc from_postfix2' ((φ_a.conj φ_b).to_postfix ++ l₁) l₂ 
-        = from_postfix2' ( φ_a.to_postfix ++ φ_b.to_postfix ++ [1] ++ l₁ ) l₂: by trivial
-    ... = from_postfix2' ( φ_a.to_postfix ++ ( φ_b.to_postfix ++ ( 1 :: l₁ ) ) ) l₂: by simp[list.append_assoc]
-    ... = from_postfix2' ( φ_b.to_postfix ++ (1 :: l₁) ) (φ_a :: l₂) : φ_ih_a
-    ... = from_postfix2' ( 1 :: l₁ ) ( φ_b :: φ_a :: l₂) : φ_ih_b
-    ... = from_postfix2' l₁ (φ_a.conj φ_b :: l₂) : by trivial,
+    calc from_postfix' ((φ_a.conj φ_b).to_postfix ++ l₁) l₂
+        = from_postfix' ( φ_a.to_postfix ++ φ_b.to_postfix ++ [1] ++ l₁ ) l₂: by trivial
+    ... = from_postfix' ( φ_a.to_postfix ++ ( φ_b.to_postfix ++ ( 1 :: l₁ ) ) ) l₂: by simp[list.append_assoc]
+    ... = from_postfix' ( φ_b.to_postfix ++ (1 :: l₁) ) (φ_a :: l₂) : φ_ih_a
+    ... = from_postfix' ( 1 :: l₁ ) ( φ_b :: φ_a :: l₂) : φ_ih_b
+    ... = from_postfix' l₁ (φ_a.conj φ_b :: l₂) : by trivial,
   }, {
     intros l₁ l₂,
     specialize φ_ih_a (φ_b.to_postfix ++ (2 :: l₁) ) l₂,
     specialize φ_ih_b (2 :: l₁) (φ_a :: l₂),
-    calc from_postfix2' ((φ_a.disj φ_b).to_postfix ++ l₁) l₂ 
-        = from_postfix2' ( φ_a.to_postfix ++ φ_b.to_postfix ++ [2] ++ l₁ ) l₂: by trivial
-    ... = from_postfix2' ( φ_a.to_postfix ++ ( φ_b.to_postfix ++ ( 2 :: l₁ ) ) ) l₂: by simp[list.append_assoc]
-    ... = from_postfix2' ( φ_b.to_postfix ++ (2 :: l₁) ) (φ_a :: l₂) : φ_ih_a
-    ... = from_postfix2' ( 2 :: l₁ ) ( φ_b :: φ_a :: l₂) : φ_ih_b
-    ... = from_postfix2' l₁ (φ_a.disj φ_b :: l₂) : by trivial,
+    calc from_postfix' ((φ_a.disj φ_b).to_postfix ++ l₁) l₂
+        = from_postfix' ( φ_a.to_postfix ++ φ_b.to_postfix ++ [2] ++ l₁ ) l₂: by trivial
+    ... = from_postfix' ( φ_a.to_postfix ++ ( φ_b.to_postfix ++ ( 2 :: l₁ ) ) ) l₂: by simp[list.append_assoc]
+    ... = from_postfix' ( φ_b.to_postfix ++ (2 :: l₁) ) (φ_a :: l₂) : φ_ih_a
+    ... = from_postfix' ( 2 :: l₁ ) ( φ_b :: φ_a :: l₂) : φ_ih_b
+    ... = from_postfix' l₁ (φ_a.disj φ_b :: l₂) : by trivial,
   }, {
     intros l₁ l₂,
     specialize φ_ih (0 :: l₁) l₂,
-    calc from_postfix2' ( (φ_a.not).to_postfix ++ l₁) l₂ 
-        = from_postfix2' ( φ_a.to_postfix ++ [0] ++ l₁ ) l₂: by trivial
-    ... = from_postfix2' ( φ_a.to_postfix ++ ( 0 :: l₁ ) ) l₂: by simp[list.append_assoc]
-    ... = from_postfix2' ( 0 :: l₁ ) ( φ_a :: l₂) : φ_ih
-    ... = from_postfix2' l₁ (φ_a.not :: l₂) : by trivial,
+    calc from_postfix' ( (φ_a.not).to_postfix ++ l₁) l₂
+        = from_postfix' ( φ_a.to_postfix ++ [0] ++ l₁ ) l₂: by trivial
+    ... = from_postfix' ( φ_a.to_postfix ++ ( 0 :: l₁ ) ) l₂: by simp[list.append_assoc]
+    ... = from_postfix' ( 0 :: l₁ ) ( φ_a :: l₂) : φ_ih
+    ... = from_postfix' l₁ (φ_a.not :: l₂) : by trivial,
   },
 end
 
@@ -166,9 +171,9 @@ end propositional_formula
 
 namespace encodable
 open propositional_formula
-instance propositional_formula_nat : encodable (propositional_formula ℕ) := { 
+instance propositional_formula_nat : encodable (propositional_formula ℕ) := {
   encode := encodable.list.encode ∘ to_postfix,
-  decode := ( option.domain_add_option from_postfix2 ) ∘ encodable.list.decode,
+  decode := ( option.domain_add_option from_postfix ) ∘ encodable.list.decode,
   encodek := begin
     intro φ,
     repeat {rw comp_app},
@@ -177,7 +182,7 @@ instance propositional_formula_nat : encodable (propositional_formula ℕ) := {
     rw el,
     simp,
     clear el,
-    change list.head' ( from_postfix2' (to_postfix φ) [] ).2 = some φ,
+    change list.head' ( from_postfix' (to_postfix φ) [] ).2 = some φ,
     let from_to_postfix_id := from_to_postfix_id_aux φ [] [],
     simp at from_to_postfix_id,
     rw from_to_postfix_id,
@@ -185,55 +190,15 @@ instance propositional_formula_nat : encodable (propositional_formula ℕ) := {
   end,
 }
 end encodable
-
-namespace primcodable 
-open propositional_formula
-instance propositional_formula_nat : primcodable (propositional_formula ℕ) := { 
-  prim := begin
-    let enc := λ a, nat.succ (encodable.encode_list ( to_postfix a )),
-    let dec := λ n, option.domain_add_option from_postfix2 ( encodable.decode_list n ),
-    change nat.primrec (λ n, 
-      option.cases_on (dec n) 
-        0 
-        enc ),
-    --have none_decidable : decidable ( dec n = none ),
-    change nat.primrec (λ n, 
-      if h : (dec n).is_none then 0 else enc ( dec n ) ),
-
-  end,
-  ..encodable.propositional_formula_nat,
-}
-
-end primcodable
-
-
-
-instance prop_prim : primcodable (propositional_formula ℕ) := { 
-  encode := encodable.list.encode ∘ propositional_formula.to_postfix,
-  decode := ( option.domain_add_option propositional_formula.from_postfix ) ∘ encodable.list.decode,
-  encodek := begin
-    intro φ,
-    repeat {rw comp_app},
-    let el := encodable.list.encodek,
-    specialize el φ.to_postfix,
-    rw el,
-    simp,
-    clear el,
-    induction φ, {
-      calc propositional_formula.from_postfix (propositional_formula.atom φ).to_postfix = some atom φ
-    },
-  end,
-  prim := _ }
-
 -- End postfix territory
 
 
 -- note that singleton a = a is also a rec_list (but not a list)
-inductive rec_list (α : Type*)
-| nil : rec_list
-| singleton (a:α) : rec_list
-| singlelist (a : rec_list) : rec_list
-| cons (hd : rec_list) (tl : rec_list) : rec_list -- think of this as [hd] concatenated with tl
+-- inductive rec_list (α : Type*)
+-- | nil : rec_list
+-- | singleton (a:α) : rec_list
+-- | singlelist (a : rec_list) : rec_list
+-- | cons (hd : rec_list) (tl : rec_list) : rec_list -- think of this as [hd] concatenated with tl
 
 namespace propositional_formula
 def eval {α : Type*} (f : α → Prop) : (propositional_formula α) → Prop
@@ -242,15 +207,17 @@ def eval {α : Type*} (f : α → Prop) : (propositional_formula α) → Prop
   | (disj a b) := (eval a) ∨ (eval b)
   | (not a) := ¬(eval a)
 
-notation h :: t  := rec_list.cons h t
-notation `[` l:(foldr `, ` (h t, rec_list.cons h t) rec_list.nil `]`) := l
+-- propositional_formula.eval a = run tm_van_Daan (encode a)
 
--- def encode_to_list {α : Type*} [h: primcodable α]: (propositional_formula α) → list ℕ
-def encode_to_list : (propositional_formula ℕ) → rec_list ℕ
-  | (atom a) := rec_list.singleton a
-  | (conj a b) := [(encode_to_list a),rec_list.singleton 0,(encode_to_list b)]
-  | (disj a b) := [(encode_to_list a),rec_list.singleton 1,(encode_to_list b)]
-  | (not a) := [rec_list.singleton 0,(encode_to_list a)]
+-- notation h :: t  := rec_list.cons h t
+-- notation `[` l:(foldr `, ` (h t, rec_list.cons h t) rec_list.nil `]`) := l
+
+-- -- def encode_to_list {α : Type*} [h: primcodable α]: (propositional_formula α) → list ℕ
+-- def encode_to_list : (propositional_formula ℕ) → rec_list ℕ
+--   | (atom a) := rec_list.singleton a
+--   | (conj a b) := [(encode_to_list a),rec_list.singleton 0,(encode_to_list b)]
+--   | (disj a b) := [(encode_to_list a),rec_list.singleton 1,(encode_to_list b)]
+--   | (not a) := [rec_list.singleton 0,(encode_to_list a)]
 
 -- def decode_from_list : rec_list ℕ → option (propositional_formula ℕ)
 --   | rec_list.nil : begin
@@ -260,10 +227,45 @@ end propositional_formula
 def is_satisfiable {α : Type*} (p : propositional_formula α) : Prop :=
 ∃ f : α → Prop, p.eval f
 
-instance prop_prim : primcodable (propositional_formula ℕ) := sorry
-
 def sat : problem (propositional_formula ℕ) :=
 { yesinstance := λ p, is_satisfiable p }
+
+@[derive [decidable_eq, inhabited]]
+inductive Γ' | blank | bit0 | bit1
+
+def tr_pos_num : pos_num → list Γ'
+| pos_num.one := [Γ'.bit1]
+| (pos_num.bit0 n) := Γ'.bit0 :: tr_pos_num n
+| (pos_num.bit1 n) := Γ'.bit1 :: tr_pos_num n
+
+def tr_num : num → list Γ'
+| num.zero := []
+| (num.pos n) := tr_pos_num n
+
+def tr_nat (n : ℕ) : list Γ' := tr_num n
+
+structure tm0 :=
+(Λ : Type*)
+(Λ_inhabited : inhabited Λ)
+(machine : turing.TM0.machine Γ' Λ) --Λ → Γ → turing.TM0.stmt Γ)
+
+#check @turing.TM0.eval
+
+example (α : Type*) (S : setoid α) (a : α) : quotient S :=
+begin
+  refine ⟦a⟧,
+end
+
+def list_to_list_blank {Γ : Type} [inhabited Γ] (L : list Γ) : turing.list_blank Γ :=
+@quotient.mk (list Γ) (turing.blank_rel.setoid Γ) L
+
+def run {α : Type*} [encodable α] (tm : tm0) (a : α) : roption (turing.list_blank Γ') :=
+@turing.TM0.eval Γ' _ tm.Λ tm.Λ_inhabited tm.machine (tr_nat (encodable.encode a))
+
+def solved_by_turing_machine {α : Type*} [encodable α] (P : problem α) (tm : tm0) : Prop := (λ (a : α), run tm a = roption.some (list_to_list_blank [Γ'.bit1])) = P.yesinstance ∧ ∀ (a : α), run tm a ≠ roption.none
+
+def solvable {α : Type*} [encodable α] (P : problem α) : Prop :=
+∃ (tm : tm0), solved_by_turing_machine P tm
 
 
 
